# 推导3(not finished)

$$
L(a_2) = f(1,1)+2f(1,2)+f(2,2) \\
+2\sum_{j=3}^Nf(1,j) +2\sum_{j=3}^Nf(2,j) \\
-a_1 - a_2 + 常数项\tag {1}
$$
其中：  
$$
f(i, j) = a_ia_jy_iy_jK_{ij}   \\
a_1 = \frac {-\xi - a_2y_2}{y_1}
$$
$$K_{ij}$$是预先计算好的值，也看作是常数

公式（3）对$$a_2$$求导，并令导数为0，得到$$a_2$$的值  

已知：  
$$
\frac{\partial a_1}{\partial a_2} = \frac{\partial \frac {-\xi - a_2y_2}{y_1}}{\partial a_2} = -\frac{y_2}{y_1} \tag {2}
$$
$$
\frac{\partial f(1,1)}{\partial a_2} = \frac{\partial a_1^2K_{11}}{\partial a_1}\frac{\partial a_1}{\partial a_2} = -2K_{11}a_1\frac{y_2}{y_1} \\
= 2K_{11}y_2\xi + 2K_{11}a_2    \tag {3}
$$
$$
f(1,2) = a_1a_2y_1y_2K_{12} = \frac {-\xi - a_2y_2}{y_1}a_2y_1y_2K_{12} = -\xi y_2K_{12}a_2 - K_{12}a_2^2   \\
\frac{\partial f(1,2)}{\partial a_2} = \frac{\partial (-\xi y_2K_{12}a_2 - K_{12}a_2^2))}{\partial a_2} = -\xi y_2K_{12} - 2K_{12}a_2 \tag {4}
$$
$$
\frac{\partial f(2,2)}{\partial a_2} = \frac{\partial a_2^2K22}{\partial a_2} = 2K_{22}a_2 \tag {5}
$$
$$
\frac{\partial \sum_{j=3}^Nf(1,j)}{\partial a_2} = \frac{\partial \sum_{j=3}^Na_1a_jy_1y_jK_{1j}}{\partial a_1}\frac{\partial a_1}{\partial a_2} \\
= \sum_{j=3}^Na_jy_1y_jK_{1j} (-\frac{y_2}{y_1}) \\
= -y_2\sum_{j=3}^Na_jy_jK_{1j} \tag {6}
$$
$$
\frac{\partial \sum_{j=3}^Nf(2,j)}{\partial a_2} = \frac{\partial \sum_{j=3}^Na_2a_jy_2y_jK_{2j}}{\partial a_2}
= \sum_{j=3}^Na_jy_2y_jK_{2j} \tag {7}
$$

得：  
$$
\frac{\partial L(a_2)}{\partial a_2} = \frac{\partial f(1,1)}{\partial a_2} + 2\frac{\partial f(1,2)}{\partial a_2} + \frac{\partial f(2,2)}{\partial a_2} + 2\frac{\partial \sum_{j=3}^Nf(1,j)}{\partial a_2} + 2\frac{\partial \sum_{j=3}^Nf(2,j)}{\partial a_2} - \frac{\partial a_1}{\partial a_2} - 1
= {...} \tag {8}
$$

令公式（8）等于0，解得的$$a_2$$为更新后的$$a_2^{new}$$  
$$
a_2^{new} = a_2^{old} + \frac{y_2(E_1-E_2)}{K_{11}+K_{12}-2K_{12}}
$$